WIP

share/pulse/examples/dice/cbor/CDDL.Spec.MapGroupGen2.fsti
@@ -37,6 +37,15 @@ val ghost_map_equiv (#key #value: Type) (f1 f2: ghost_map key value) : Lemma
 let ghost_map_defined (#key #value: Type) (k: key) (f: ghost_map key value) : Tot prop =
   Some? (apply_ghost_map f k)
 
+let ghost_map_defined_alt
+  (#key #value: Type) (k: key) (f: ghost_map key value)
+: Lemma
+  (ghost_map_defined k f <==> (exists v . ghost_map_mem (k, v) f))
+  [SMTPat (ghost_map_defined k f)]
+= match apply_ghost_map f k with
+  | None -> ()
+  | Some _ -> ()
+
 let ghost_map_disjoint (#key #value1 #value2: Type) (f1: ghost_map key value1) (f2: ghost_map key value2) : Tot prop =
   (forall k . ~ (ghost_map_defined k f1 /\ ghost_map_defined k f2))
 
@@ -62,6 +71,16 @@ val apply_ghost_map_union (#key #value: Type) (m1 m2: ghost_map key value) (k: k
   end)
   [SMTPat (apply_ghost_map (ghost_map_union m1 m2) k)]
 
+let ghost_map_union_empty_l (#key #value: Type) (m: ghost_map key value) : Lemma
+  (ghost_map_union ghost_map_empty m == m)
+  [SMTPat (ghost_map_union ghost_map_empty m)]
+= ghost_map_ext (ghost_map_union ghost_map_empty m) m
+
+let ghost_map_union_empty_r (#key #value: Type) (m: ghost_map key value) : Lemma
+  (ghost_map_union m ghost_map_empty == m)
+  [SMTPat (ghost_map_union m ghost_map_empty)]
+= ghost_map_ext (ghost_map_union m ghost_map_empty) m
+
 let ghost_map_disjoint_mem_union (#key #value: Type) (m1 m2: ghost_map key value) (xv: (key & value)) : Lemma
   (requires ghost_map_disjoint m1 m2)
   (ensures ghost_map_mem xv (m1 `ghost_map_union` m2) <==> ghost_map_mem xv m1 \/ ghost_map_mem xv m2)
@@ -74,6 +93,21 @@ let ghost_map_disjoint_mem_union' (#key #value: Type) (m1 m2: ghost_map key valu
 val ghost_map_disjoint_union (#key #value: Type) (m1 m2: ghost_map key value) : Lemma
   (requires ghost_map_disjoint m1 m2)
   (ensures m1 `ghost_map_union` m2 == m2 `ghost_map_union` m1)
+
+val ghost_map_length (#key #value: Type) (m: ghost_map key value) : GTot nat
+
+val ghost_map_length_empty (key value: Type) : Lemma
+  (ghost_map_length (ghost_map_empty #key #value) == 0)
+  [SMTPat (ghost_map_length (ghost_map_empty #key #value))]
+
+val ghost_map_length_singleton (#key #value: Type) (k: key) (v: value) : Lemma
+  (ghost_map_length (ghost_map_singleton k v) == 1)
+  [SMTPat (ghost_map_length (ghost_map_singleton k v))]
+
+val ghost_map_length_disjoint_union (#key #value: Type) (m1 m2: ghost_map key value) : Lemma
+  (requires ghost_map_disjoint m1 m2)
+  (ensures (ghost_map_length (ghost_map_union m1 m2) == ghost_map_length m1 + ghost_map_length m2))
+  [SMTPat (ghost_map_length (ghost_map_union m1 m2))]
 
 let map_group_item_post
   (l: ghost_map Cbor.raw_data_item Cbor.raw_data_item)
@@ -142,6 +176,24 @@ val apply_ghost_map_filter
   end)
   [SMTPat (apply_ghost_map (ghost_map_filter f m) k)]
 
+let ghost_map_mem_filter
+  (#key #value: Type)
+  (f: (key & value) -> GTot bool)
+  (m: ghost_map key value)
+  (x: (key & value))
+: Lemma
+  (ghost_map_mem x (ghost_map_filter f m) <==> ghost_map_mem x m /\ f x)
+= ()
+
+let ghost_map_filter_for_all
+  (#key #value: Type)
+  (f: (key & value) -> GTot bool)
+  (m: ghost_map key value)
+: Lemma
+  (requires forall x . ghost_map_mem x m ==> f x)
+  (ensures ghost_map_filter f m == m)
+= ghost_map_equiv (ghost_map_filter f m) m
+
 let ghost_map_filter_ext
   (#key #value: Type)
   (f1 f2: (key & value) -> GTot bool)
@@ -150,6 +202,17 @@ let ghost_map_filter_ext
   (requires forall x . f1 x == f2 x)
   (ensures ghost_map_filter f1 m == ghost_map_filter f2 m)
 = ghost_map_equiv (ghost_map_filter f1 m) (ghost_map_filter f2 m)
+
+let ghost_map_disjoint_union_filter
+  (#key #value: Type)
+  (f: (key & value) -> GTot bool)
+  (m1 m2: ghost_map key value)
+: Lemma
+  (requires ghost_map_disjoint m1 m2)
+  (ensures (ghost_map_filter f (ghost_map_union m1 m2) == ghost_map_filter f m1 `ghost_map_union` ghost_map_filter f m2))
+= ghost_map_ext
+    (ghost_map_filter f (ghost_map_union m1 m2))
+    (ghost_map_filter f m1 `ghost_map_union` ghost_map_filter f m2)
 
 val ghost_map_of_list
   (#key #value: Type)
@@ -190,6 +253,14 @@ val ghost_map_filter_of_list
   (l: list (key & value) { List.Tot.no_repeats_p (List.Tot.map fst l) })
 : Lemma
   (ghost_map_filter f (ghost_map_of_list l) == ghost_map_of_list (List.Tot.filter f l))
+
+val ghost_map_length_of_list
+  (#key #value: Type)
+  (l: list (key & value))
+: Lemma
+  (requires List.Tot.no_repeats_p (List.Tot.map fst l))
+  (ensures ghost_map_length (ghost_map_of_list l) == List.Tot.length l)
+  [SMTPat (ghost_map_length (ghost_map_of_list l))]
 
 val map_group_zero_or_more_zero_or_one_eq
   (m: map_group)
@@ -315,6 +386,26 @@ let rec list_filter_filter (#t: Type) (p1 p2: t -> bool) (l: list t) : Lemma
   | [] -> ()
   | a :: q -> list_filter_filter p1 p2 q
 
+let ghost_map_filter_filter
+  (#key #value: Type)
+  (p1 p2: (key & value) -> GTot bool)
+  (f: ghost_map key value)
+: Lemma
+  (ghost_map_filter p2 (ghost_map_filter p1 f) == ghost_map_filter (p1 `andp_g` p2) f)
+= ghost_map_equiv
+    (ghost_map_filter p2 (ghost_map_filter p1 f))
+    (ghost_map_filter (p1 `andp_g` p2) f)
+
+let ghost_map_filter_implies
+  (#key #value: Type)
+  (p1 p2: (key & value) -> GTot bool)
+  (f: ghost_map key value)
+: Lemma
+  (requires (forall kv . p1 kv ==> p2 kv))
+  (ensures (ghost_map_filter p2 (ghost_map_filter p1 f) == ghost_map_filter p1 f))
+= ghost_map_filter_filter p1 p2 f;
+  ghost_map_filter_ext p1 (p1 `andp_g` p2) f
+
 val map_group_filter_filter (p1 p2: (Cbor.raw_data_item & Cbor.raw_data_item) -> GTot bool) : Lemma
   (map_group_filter p1 `map_group_concat` map_group_filter p2 == map_group_filter (andp_g p1 p2))
   [SMTPat (map_group_filter p1 `map_group_concat` map_group_filter p2)]
@@ -400,10 +491,725 @@ val matches_map_group_det (g: map_group) (m: list (Cbor.raw_data_item & Cbor.raw
   | MapGroupFail -> ~ (matches_map_group g m)
   | MapGroupDet _ m' -> matches_map_group g m <==> m' == ghost_map_empty
   | _ -> True)
+  [SMTPat (matches_map_group g m)]
 
-let t_map (g: map_group) : typ =
-  fun x -> match x with
-  | Cbor.Map m -> 
-//    FStar.StrongExcludedMiddle.strong_excluded_middle (List.Tot.no_repeats_p (List.Tot.map fst m)) &&
-    matches_map_group g m
-  | _ -> false
+val t_map (g: map_group) : typ
+
+val t_map_eq
+  (g: map_group)
+  (x: Cbor.raw_data_item)
+: Lemma
+  (t_map g x == true <==> begin match x with
+    | Cbor.Map m ->
+      List.Tot.no_repeats_p (List.Tot.map fst m) /\
+      matches_map_group g m
+    | _ -> False
+  end)
+  [SMTPat (t_map g x)]
+
+
+let det_map_group = (m: map_group { forall l . ~ (MapGroupNonDet? (apply_map_group_det m l)) })
+
+let map_group_parser_spec_arg
+  (source: det_map_group)
+  (#target: Type0)
+  (target_size: target -> nat)
+: Tot Type0
+= (x: list (Cbor.raw_data_item & Cbor.raw_data_item) { // list needed because I need to preserve the order of elements when parsing a table
+    List.Tot.no_repeats_p (List.Tot.map fst x) /\
+    begin match apply_map_group_det source (ghost_map_of_list x) with
+    | MapGroupDet _ rem -> rem == ghost_map_empty
+    | _ -> False
+    end
+  })
+
+let map_group_parser_spec_ret
+  (source: det_map_group)
+  (#target: Type0)
+  (target_size: target -> nat)
+  (x: map_group_parser_spec_arg source target_size)
+: Tot Type0
+= (y: target { 
+    target_size y == List.Tot.length x
+  })
+
+let map_group_parser_spec
+  (source: det_map_group)
+  (#target: Type0)
+  (target_size: target -> nat)
+: Type0
+= (x: map_group_parser_spec_arg source target_size) -> GTot (map_group_parser_spec_ret source target_size x)
+
+let map_group_serializer_spec
+  (#source: det_map_group)
+  (#target: Type0)
+  (#target_size: target -> nat)
+  (p: map_group_parser_spec source target_size)
+  (target_guard: (Cbor.raw_data_item & Cbor.raw_data_item) -> Tot prop) // to take cuts into account. This implies that it is the responsibility of the designer of the target type to make sure entries violating cuts are not introduced.
+: Type0
+= (x: target) -> GTot (y: list (Cbor.raw_data_item & Cbor.raw_data_item) {
+    List.Tot.no_repeats_p (List.Tot.map fst y) /\
+    matches_map_group source y /\
+    p y == x /\
+    (forall z . List.Tot.memP z y ==> target_guard z)
+  })
+
+let map_group_target_serializable
+  (#target: Type0)
+  (target_size: target -> nat)
+: Tot Type0
+= (x: target { target_size x < pow2 64 })
+
+let parser_spec_map_group
+  (#source: det_map_group)
+  (#target: Type0)
+  (#target_size: target -> nat)
+  (p: map_group_parser_spec source target_size)
+: Tot (parser_spec (t_map source) (map_group_target_serializable target_size))
+= fun x ->
+    let Cbor.Map a = x in
+    let res = p a in
+    res
+
+let serializer_spec_map_group
+  (#source: det_map_group)
+  (#target: Type0)
+  (#target_size: target -> nat)
+  (#p: map_group_parser_spec source target_size)
+  (#target_guard: (Cbor.raw_data_item & Cbor.raw_data_item) -> Tot prop)
+  (s: map_group_serializer_spec p target_guard)
+: Tot (serializer_spec (parser_spec_map_group p))
+= fun x -> Cbor.Map (s x)
+
+let map_group_parser_spec_bij
+  (#source: det_map_group)
+  (#target1: Type0)
+  (#target_size1: target1 -> nat)
+  (f: map_group_parser_spec source target_size1)
+  (#target2: Type0)
+  (target_size2: target2 -> nat)
+  (bij: bijection target1 target2 {
+    forall x2 . target_size2 x2 == target_size1 (bij.bij_to_from x2)
+  })
+: Tot (map_group_parser_spec source target_size2)
+= fun x -> bij.bij_from_to (f x)
+
+let map_group_serializer_spec_bij
+  (#source: det_map_group)
+  (#target1: Type0)
+  (#target_size1: target1 -> nat)
+  (#f: map_group_parser_spec source target_size1)
+  (#target_guard: (Cbor.raw_data_item & Cbor.raw_data_item) -> Tot prop)
+  (s: map_group_serializer_spec f target_guard)
+  (#target2: Type0)
+  (target_size2: target2 -> nat)
+  (bij: bijection target1 target2 {
+    forall x2 . target_size2 x2 == target_size1 (bij.bij_to_from x2)
+  })
+: Tot (map_group_serializer_spec (map_group_parser_spec_bij f target_size2 bij) target_guard)
+= fun x -> s (bij.bij_to_from x)
+
+let map_group_parser_spec_match_item_for
+  (cut: bool)
+  (k: Cbor.raw_data_item)
+  (#ty: typ)
+  (#target: Type)
+  (p: parser_spec ty target)
+  (target_size: target -> nat {
+    forall x . target_size x == 1
+  })
+: Tot (map_group_parser_spec (map_group_match_item_for cut k ty) target_size)
+= fun x ->
+  ghost_map_length_of_list x;
+  let Some v = Cbor.list_ghost_assoc k x in
+  p v
+
+let map_group_serializer_spec_match_item_for
+  (#cut: bool)
+  (#k: Cbor.raw_data_item)
+  (#ty: typ)
+  (#target: Type)
+  (#p: parser_spec ty target)
+  (s: serializer_spec p)
+  (target_size: target -> nat {
+    forall x . target_size x == 1
+  })
+  (target_guard: (Cbor.raw_data_item & Cbor.raw_data_item) -> Tot prop {
+    forall v . ty v ==> target_guard (k, v)
+  })
+: Tot (map_group_serializer_spec (map_group_parser_spec_match_item_for cut k p target_size) target_guard)
+= fun x ->
+  let v = s x in
+  let res = [k, v] in
+  let mres = ghost_map_of_list res in
+  ghost_map_equiv mres (ghost_map_singleton k v);
+  let MapGroupDet _ rem = apply_map_group_det (map_group_match_item_for cut k ty) mres in
+  ghost_map_equiv rem ghost_map_empty;
+  res
+
+let map_group_parser_spec_concat_shrinkable
+  (g: map_group)
+: Tot prop
+= forall x . match apply_map_group_det g x with
+  | MapGroupDet consumed rem ->
+    forall rem1 rem2 . (
+      rem1 `ghost_map_disjoint` rem2 /\
+      rem1 `ghost_map_union` rem2 == rem
+    ) ==>
+    apply_map_group_det g (consumed `ghost_map_union` rem1) == MapGroupDet consumed rem1
+  | MapGroupFail -> // necessary for compatibility with `//` . NOTE: This does not hold for things like (?((k1=>t1)(k2=>t2)))(k1=>t'), so we will need some independence conditions, see below.
+    forall x1 x2 . x == x1 `ghost_map_union` x2 ==>
+    (MapGroupFail? (apply_map_group_det g x1) \/ MapGroupCutFail? (apply_map_group_det g x1))
+  | _ -> True
+
+#restart-solver
+let map_group_parser_spec_concat_shrinkable_intro
+  (g: map_group)
+  (prf: (x: _) -> (rem1: _) -> (rem2: _) -> Lemma
+    (requires (
+      match apply_map_group_det g x with
+      | MapGroupDet consumed rem ->
+        rem1 `ghost_map_disjoint` rem2 /\
+        rem1 `ghost_map_union` rem2 == rem /\
+        consumed `ghost_map_disjoint` rem1 /\
+        consumed `ghost_map_disjoint` rem2
+      | _ -> False
+    ))
+    (ensures (
+      match apply_map_group_det g x with
+      | MapGroupDet consumed _ ->
+        apply_map_group_det g (consumed `ghost_map_union` rem1) == MapGroupDet consumed rem1
+      | _ -> True
+    ))
+  )
+  (prf2: (x1: _) -> (x2: _) -> Lemma
+    (requires MapGroupFail? (apply_map_group_det g (x1 `ghost_map_union` x2)))
+    (ensures MapGroupFail? (apply_map_group_det g x1) \/ MapGroupCutFail? (apply_map_group_det g x1))
+  )
+(*
+  (prf3: (x1: _) -> (x2: _) -> Lemma
+    (requires MapGroupCutFail? (apply_map_group_det g x1))
+    (ensures MapGroupCutFail? (apply_map_group_det g (x1 `ghost_map_union` x2)))
+  )
+*)  
+: Lemma
+  (map_group_parser_spec_concat_shrinkable g)
+= Classical.forall_intro_3 (fun rem1 rem2 -> Classical.move_requires (prf rem1 rem2));
+  Classical.forall_intro_2 (fun x1 -> Classical.move_requires (prf2 x1));
+//  Classical.forall_intro_2 (fun x1 -> Classical.move_requires (prf3 x1));
+  ()
+
+let map_group_parser_spec_concat_shrinkable_match_item_for
+  (cut: bool)
+  (k: Cbor.raw_data_item)
+  (ty: typ)
+: Lemma
+  (map_group_parser_spec_concat_shrinkable
+    (map_group_match_item_for cut k ty)
+  )
+= map_group_parser_spec_concat_shrinkable_intro (map_group_match_item_for cut k ty) (fun x rem1 rem2 ->
+    let MapGroupDet consumed rem = apply_map_group_det (map_group_match_item_for cut k ty) x in
+    let Some v = apply_ghost_map x k in
+    assert (consumed == ghost_map_singleton k v);
+    assert (apply_ghost_map consumed k == Some v);
+    assert (apply_ghost_map (consumed `ghost_map_union` rem1) k == Some v);
+    ghost_map_disjoint_union_filter (notp_g (matches_map_group_entry (t_literal k) ty)) rem1 rem2;
+    ghost_map_disjoint_union_filter (notp_g (matches_map_group_entry (t_literal k) ty)) consumed rem1;
+    ghost_map_equiv
+      (ghost_map_filter (notp_g (matches_map_group_entry (t_literal k) ty)) consumed)
+      ghost_map_empty;
+    ghost_map_filter_implies
+      (notp_g (matches_map_group_entry (t_literal k) ty))
+      (notp_g (matches_map_group_entry (t_literal k) ty))
+      rem1;
+    assert (ghost_map_filter (notp_g (matches_map_group_entry (t_literal k) ty)) (consumed `ghost_map_union` rem1) == ghost_map_filter (notp_g (matches_map_group_entry (t_literal k) ty)) consumed `ghost_map_union` ghost_map_filter (notp_g (matches_map_group_entry (t_literal k) ty)) rem1);
+    assert (ghost_map_filter (notp_g (matches_map_group_entry (t_literal k) ty)) consumed == ghost_map_empty);
+    ghost_map_filter_for_all (notp_g (matches_map_group_entry (t_literal k) ty)) rem1;
+    assert (ghost_map_filter (notp_g (matches_map_group_entry (t_literal k) ty)) rem1 == rem1);
+    assert (ghost_map_filter (notp_g (matches_map_group_entry (t_literal k) ty)) (consumed `ghost_map_union` rem1) == ghost_map_empty `ghost_map_union` rem1);
+    assert (apply_map_group_det (map_group_match_item_for cut k ty) (consumed `ghost_map_union` rem1) == MapGroupDet consumed rem1);
+    ()
+  )
+  (fun x1 x2 -> ())
+//  (fun x1 x2 -> ())
+
+let map_group_parser_spec_concat_shrinkable_elim
+  (g: map_group)
+  (x: _)
+  (rem1: _)
+  (rem2: _)
+: Lemma
+    (requires (
+      map_group_parser_spec_concat_shrinkable g /\
+      begin match apply_map_group_det g x with
+      | MapGroupDet consumed rem ->
+        rem1 `ghost_map_disjoint` rem2 /\
+        rem1 `ghost_map_union` rem2 == rem
+      | _ -> False
+      end
+    ))
+    (ensures (
+      match apply_map_group_det g x with
+      | MapGroupDet consumed _ ->
+        consumed `ghost_map_disjoint` rem1 /\
+        consumed `ghost_map_disjoint` rem2 /\
+        apply_map_group_det g (consumed `ghost_map_union` rem1) == MapGroupDet consumed rem1
+      | _ -> True
+    ))
+= ()
+
+let map_group_parser_spec_concat_shrinkable_elim_weak
+  (g: map_group)
+  (x: ghost_map Cbor.raw_data_item Cbor.raw_data_item)
+: Lemma
+  (requires map_group_parser_spec_concat_shrinkable g /\
+    MapGroupDet? (apply_map_group_det g x)
+  )
+  (ensures (match apply_map_group_det g x with
+  | MapGroupDet consumed rem ->
+    apply_map_group_det g consumed == MapGroupDet consumed ghost_map_empty
+  | _ -> True
+  ))
+= let MapGroupDet _ rem = apply_map_group_det g x in
+  map_group_parser_spec_concat_shrinkable_elim g x ghost_map_empty rem
+
+val list_extract_from_ghost_map
+  (#key #value: Type)
+  (l: list (key & value) {
+    List.Tot.no_repeats_p (List.Tot.map fst l)
+  })
+  (g': ghost_map key value { forall x . ghost_map_mem x g' ==> ghost_map_mem x (ghost_map_of_list l) })
+: GTot (l' : list (key & value) {
+    List.Tot.no_repeats_p (List.Tot.map fst l') /\
+    ghost_map_of_list l' == g'
+  })
+
+let map_group_parser_spec_concat
+  (#source1: det_map_group)
+  (#target1: Type)
+  (#target_size1: target1 -> nat)
+  (p1: map_group_parser_spec source1 target_size1 {
+    map_group_parser_spec_concat_shrinkable source1
+  })
+  (#source2: det_map_group)
+  (#target2: Type)
+  (#target_size2: target2 -> nat)
+  (p2: map_group_parser_spec source2 target_size2)
+  (target_size: (target1 & target2) -> nat {
+    forall x . target_size x == target_size1 (fst x) + target_size2 (snd x)
+  })
+: Tot (map_group_parser_spec (map_group_concat source1 source2) target_size)
+= fun l ->
+  let MapGroupDet consumed1 rem1 = apply_map_group_det source1 (ghost_map_of_list l) in
+  let l1 = list_extract_from_ghost_map l consumed1 in
+  map_group_parser_spec_concat_shrinkable_elim_weak source1 (ghost_map_of_list l);
+  let res1 = p1 l1 in
+  let l2 = list_extract_from_ghost_map l rem1 in
+  let res2 = p2 l2 in
+  List.Tot.append_length l1 l2;
+  ghost_map_length_of_list l1;
+  ghost_map_length_of_list l2;
+  ghost_map_length_disjoint_union consumed1 rem1;
+  (res1, res2)
+
+let map_group_parser_spec_concat_extensible
+  (g1: map_group)
+  (target_guard2: (Cbor.raw_data_item & Cbor.raw_data_item) -> Tot prop)
+: Tot prop
+= map_group_parser_spec_concat_shrinkable g1 /\ (
+  forall l1 l2 .
+    (forall x2 . ghost_map_mem x2 l2 ==> target_guard2 x2) ==>
+    begin match apply_map_group_det g1 l1 with
+    | MapGroupDet _ rem1 ->
+      rem1 == ghost_map_empty ==> (
+        ghost_map_disjoint l1 l2 /\
+        apply_map_group_det g1 (l1 `ghost_map_union` l2) == MapGroupDet l1 l2
+      )
+    | MapGroupCutFail ->
+      MapGroupCutFail? (apply_map_group_det g1 (l1 `ghost_map_union` l2))
+    | MapGroupFail ->
+      MapGroupFail? (apply_map_group_det g1 (l1 `ghost_map_union` l2))
+    | _ -> True
+    end
+  )
+
+let map_group_parser_spec_concat_extensible_intro
+  (g1: map_group)
+  (target_guard2: (Cbor.raw_data_item & Cbor.raw_data_item) -> Tot prop)
+  (prf: (l1: _) -> (l2: _) -> Lemma
+    (requires (
+      (forall x2 . ghost_map_mem x2 l2 ==> target_guard2 x2) /\
+      begin match apply_map_group_det g1 l1 with
+      | MapGroupDet _ rem1 ->
+        rem1 == ghost_map_empty /\
+        (forall x2 . ghost_map_mem x2 l2 ==> target_guard2 x2)
+      | MapGroupNonDet -> False
+      | _ -> True
+      end
+    ))
+    (ensures (
+      let res = apply_map_group_det g1 (l1 `ghost_map_union` l2) in
+      begin match apply_map_group_det g1 l1 with
+      | MapGroupDet _ _ ->
+        ghost_map_disjoint l1 l2 /\
+        res == MapGroupDet l1 l2
+      | MapGroupCutFail -> MapGroupCutFail? res
+      | MapGroupFail -> MapGroupFail? res
+      | _ -> True
+      end
+    ))
+  )
+: Lemma
+  (requires map_group_parser_spec_concat_shrinkable g1)
+  (ensures map_group_parser_spec_concat_extensible g1 target_guard2)
+= Classical.forall_intro_2 (fun l1 -> Classical.move_requires (prf l1))
+
+let map_group_parser_spec_concat_extensible_match_item_for
+  (cut: bool)
+  (k: Cbor.raw_data_item)
+  (ty: typ)
+  (target_guard: (Cbor.raw_data_item & Cbor.raw_data_item) -> prop)
+: Lemma
+  (requires
+    (forall x . target_guard x ==> (~ (fst x == k)))
+  )
+  (ensures map_group_parser_spec_concat_extensible
+    (map_group_match_item_for cut k ty) target_guard
+  )
+= map_group_parser_spec_concat_shrinkable_match_item_for cut k ty;
+  map_group_parser_spec_concat_extensible_intro
+    (map_group_match_item_for cut k ty)
+    target_guard
+    (fun l1 l2 ->
+      match apply_ghost_map l1 k with
+      | Some v ->
+        if ty v
+        then begin
+          assert (l1 == ghost_map_singleton k v);
+          assert (ghost_map_disjoint l1 l2);
+          assert (MapGroupDet?(apply_map_group_det
+            (map_group_match_item_for cut k ty)
+            (l1 `ghost_map_union` l2)));
+          let MapGroupDet l1' l2' = apply_map_group_det
+            (map_group_match_item_for cut k ty)
+            (l1 `ghost_map_union` l2) in
+          assert (l1 == l1');
+          ghost_map_disjoint_union_filter (notp_g (matches_map_group_entry (t_literal k) ty)) l1 l2;
+          ghost_map_ext (ghost_map_filter (notp_g (matches_map_group_entry (t_literal k) ty)) l1) ghost_map_empty;
+          ghost_map_filter_for_all (notp_g (matches_map_group_entry (t_literal k) ty)) l2;
+          assert (l2 == l2')
+        end else begin
+          ()
+        end
+      | _ ->
+        assert (~ (ghost_map_defined k l2))
+    )
+
+val list_extract_from_ghost_map_append_l
+  (#key #value: Type)
+  (l1: list (key & value) {
+    List.Tot.no_repeats_p (List.Tot.map fst l1)
+  })
+  (l2: list (key & value) {
+    List.Tot.no_repeats_p (List.Tot.map fst l2)
+  })
+: Lemma
+  (requires
+    ghost_map_disjoint (ghost_map_of_list l1) (ghost_map_of_list l2)
+  )
+  (ensures
+    List.Tot.no_repeats_p (List.Tot.map fst (l1 `List.Tot.append` l2)) /\
+    (forall x . ghost_map_mem x (ghost_map_of_list l1) ==> ghost_map_mem x (ghost_map_of_list (l1 `List.Tot.append` l2))) /\
+    list_extract_from_ghost_map
+      (l1 `List.Tot.append` l2)
+      (ghost_map_of_list l1)
+    == l1
+  )
+
+val list_extract_from_ghost_map_append_r
+  (#key #value: Type)
+  (l1: list (key & value) {
+    List.Tot.no_repeats_p (List.Tot.map fst l1)
+  })
+  (l2: list (key & value) {
+    List.Tot.no_repeats_p (List.Tot.map fst l2)
+  })
+: Lemma
+  (requires
+    ghost_map_disjoint (ghost_map_of_list l1) (ghost_map_of_list l2)
+  )
+  (ensures
+    List.Tot.no_repeats_p (List.Tot.map fst (l1 `List.Tot.append` l2)) /\
+    (forall x . ghost_map_mem x (ghost_map_of_list l2) ==> ghost_map_mem x (ghost_map_of_list (l1 `List.Tot.append` l2))) /\
+    list_extract_from_ghost_map
+      (l1 `List.Tot.append` l2)
+      (ghost_map_of_list l2)
+    == l2
+  )
+
+let map_group_parser_spec_concat_extensible_elim
+  (g1: map_group)
+  (target_guard2: (Cbor.raw_data_item & Cbor.raw_data_item) -> Tot prop {
+    map_group_parser_spec_concat_extensible g1 target_guard2
+  })
+  (l1: _)
+  (consumed1: _ {
+    apply_map_group_det g1 l1 == MapGroupDet consumed1 ghost_map_empty
+  })
+  (l2: _)
+  (sq: squash (forall x2 . ghost_map_mem x2 l2 ==> target_guard2 x2))
+: Lemma (
+    ghost_map_disjoint l1 l2 /\
+    apply_map_group_det g1 (l1 `ghost_map_union` l2) == MapGroupDet l1 l2
+  )
+= ()
+
+let map_group_serializer_spec_concat
+  (#source1: det_map_group)
+  (#target1: Type)
+  (#target_size1: target1 -> nat)
+  (#p1: map_group_parser_spec source1 target_size1)
+  (#target_guard1: (Cbor.raw_data_item & Cbor.raw_data_item) -> Tot prop)
+  (s1: map_group_serializer_spec p1 target_guard1)
+  (#source2: det_map_group)
+  (#target2: Type)
+  (#target_size2: target2 -> nat)
+  (#p2: map_group_parser_spec source2 target_size2)
+  (#target_guard2: (Cbor.raw_data_item & Cbor.raw_data_item) -> Tot prop)
+  (s2: map_group_serializer_spec p2 target_guard2 {
+    map_group_parser_spec_concat_extensible source1 target_guard2
+  })
+  (target_size: (target1 & target2) -> nat {
+    forall x . target_size x == target_size1 (fst x) + target_size2 (snd x)
+  })
+  (target_guard: (Cbor.raw_data_item & Cbor.raw_data_item) -> Tot prop {
+    forall x . (target_guard1 x \/ target_guard2 x) ==> target_guard x
+  })
+: Tot (map_group_serializer_spec (map_group_parser_spec_concat p1 p2 target_size) target_guard)
+= fun x ->
+    let (x1, x2) = x in
+    let l1 = s1 x1 in
+    let l2 = s2 x2 in
+    List.Tot.append_length l1 l2;
+    ghost_map_of_list_append l1 l2;
+    let res = l1 `List.Tot.append` l2 in
+    let MapGroupDet consumed1 _ = apply_map_group_det source1 (ghost_map_of_list l1) in
+    Classical.forall_intro (ghost_map_of_list_mem l2);
+    let sq : squash (forall x2 . ghost_map_mem x2 (ghost_map_of_list l2) ==> target_guard2 x2) = () in
+    map_group_parser_spec_concat_extensible_elim source1 target_guard2 (ghost_map_of_list l1) consumed1 (ghost_map_of_list l2) sq;
+    list_extract_from_ghost_map_append_l l1 l2;
+    list_extract_from_ghost_map_append_r l1 l2;
+    Classical.forall_intro (List.Tot.append_memP l1 l2);
+    res
+
+let rec map_group_parser_spec_zero_or_more'
+  (#source: det_map_group)
+  (#target: Type)
+  (#target_size: target -> nat)
+  (p: map_group_parser_spec source target_size {
+    map_group3_concat_unique_strong source source
+  })
+  (target_size' : list target -> nat {
+    forall (l: list target) . target_size' l == (if Nil? l then 0 else target_size (List.Tot.hd l) + target_size' (List.Tot.tl l))
+  })
+  (x: map_group_parser_spec_arg (map_group3_zero_or_more source) target_size')
+: GTot (map_group_parser_spec_ret (map_group3_zero_or_more source) target_size' x)
+  (decreases (List.Tot.length x))
+= match source x with
+  | None ->
+    assert (x == []);
+    let res : list target = [] in
+    assert (Nil? res);
+    assert (target_size' res == 0);
+    res
+  | Some (l1, l2) ->
+    if Nil? l1
+    then []
+    else begin
+      map_group3_concat_unique_weak_zero_or_more_right source source;
+      List.Tot.append_length l1 l2;
+      let q = map_group_parser_spec_zero_or_more' p target_size' l2 in
+      p l1 :: q
+    end
+
+let map_group_parser_spec_zero_or_more
+  (#source: det_map_group)
+  (#target: Type)
+  (#target_size: target -> nat)
+  (p: map_group_parser_spec source target_size {
+    map_group3_concat_unique_strong source source
+  })
+  (target_size' : list target -> nat {
+    forall (l: list target) . target_size' l == (if Nil? l then 0 else target_size (List.Tot.hd l) + target_size' (List.Tot.tl l))
+  })
+: Tot (map_group_parser_spec (map_group3_zero_or_more source) target_size')
+= map_group_parser_spec_zero_or_more' p target_size'
+
+let nonempty_map_group : Type0 =
+  (a: map_group {
+    forall l . match a l with
+    | Some (consumed, _) -> Cons? consumed
+    | _ -> True
+  })
+
+let rec map_group_serializer_spec_zero_or_more'
+  (#source: nonempty_map_group)
+  (#target: Type)
+  (#target_size: target -> nat)
+  (#p: map_group_parser_spec source target_size)
+  (s: map_group_serializer_spec p {
+    map_group3_concat_unique_strong source source
+  })
+  (target_size' : list target -> nat {
+    forall (l: list target) . target_size' l == (if Nil? l then 0 else target_size (List.Tot.hd l) + target_size' (List.Tot.tl l))
+  })
+  (x: list target)
+: GTot (y: map_group_parser_spec_arg (map_group3_zero_or_more source) target_size' {
+    map_group_parser_spec_zero_or_more p target_size' y == x
+  })
+  (decreases x)
+= match x with
+  | [] -> []
+  | a :: q ->
+    map_group3_concat_unique_weak_zero_or_more_right source source;
+    let l1 = s a in
+    let l2 = map_group_serializer_spec_zero_or_more' s target_size' q in
+    let res = l1 `List.Tot.append` l2 in
+    res
+
+let map_group_serializer_spec_zero_or_more
+  (#source: nonempty_map_group)
+  (#target: Type)
+  (#target_size: target -> nat)
+  (#p: map_group_parser_spec source target_size)
+  (s: map_group_serializer_spec p {
+    map_group3_concat_unique_strong source source
+  })
+  (target_size' : list target -> nat {
+    forall (l: list target) . target_size' l == (if Nil? l then 0 else target_size (List.Tot.hd l) + target_size' (List.Tot.tl l))
+  })
+: Tot (map_group_serializer_spec (map_group_parser_spec_zero_or_more p target_size'))
+= map_group_serializer_spec_zero_or_more' s target_size'
+
+let nelist (a: Type) : Type0 = (l: list a { Cons? l })
+
+let map_group_parser_spec_one_or_more
+  (#source: det_map_group)
+  (#target: Type)
+  (#target_size: target -> nat)
+  (p: map_group_parser_spec source target_size {
+    map_group3_concat_unique_strong source source
+  })
+  (target_size1 : list target -> nat {
+    forall (l: list target) . target_size1 l == (if Nil? l then 0 else target_size (List.Tot.hd l) + target_size1 (List.Tot.tl l))
+  })
+  (target_size2 : nelist target -> nat {
+    forall (l: nelist target) . target_size2 l == target_size1 l
+  })
+: Tot (map_group_parser_spec (map_group3_one_or_more source) target_size2)
+= fun x ->
+  map_group3_concat_unique_weak_zero_or_more_right source source;
+  let Some (l1, l2) = source x in
+  List.Tot.append_length l1 l2;
+  p l1 :: map_group_parser_spec_zero_or_more p target_size1 l2
+
+let map_group_serializer_spec_one_or_more
+  (#source: nonempty_map_group)
+  (#target: Type)
+  (#target_size: target -> nat)
+  (#p: map_group_parser_spec source target_size)
+  (s: map_group_serializer_spec p {
+    map_group3_concat_unique_strong source source
+  })
+  (target_size1 : list target -> nat {
+    forall (l: list target) . target_size1 l == (if Nil? l then 0 else target_size (List.Tot.hd l) + target_size1 (List.Tot.tl l))
+  })
+  (target_size2 : nelist target -> nat {
+    forall (l: nelist target) . target_size2 l == target_size1 l
+  })
+: Tot (map_group_serializer_spec (map_group_parser_spec_one_or_more p target_size1 target_size2))
+= fun x ->
+  map_group3_concat_unique_weak_zero_or_more_right source source;
+  let hd :: tl = x in
+  let l1 = s hd in
+  let l2 = map_group_serializer_spec_zero_or_more s target_size1 tl in
+  List.Tot.append_length l1 l2;
+  l1 `List.Tot.append` l2
+
+let map_group_parser_spec_choice
+  (#source1: det_map_group)
+  (#target1: Type0)
+  (#target_size1: target1 -> nat)
+  (p1: map_group_parser_spec source1 target_size1)
+  (#source2: det_map_group)
+  (#target2: Type0)
+  (#target_size2: target2 -> nat)
+  (p2: map_group_parser_spec source2 target_size2)
+  (target_size: (target1 `either` target2) -> nat {
+    forall x . target_size x == begin match x with
+    | Inl y -> target_size1 y
+    | Inr y -> target_size2 y
+    end
+  })
+: Tot (map_group_parser_spec (source1 `map_group3_choice` source2) target_size)
+= fun x ->
+    if Some? (source1 x)
+    then Inl (p1 x)
+    else Inr (p2 x)
+
+let map_group_serializer_spec_choice
+  (#source1: det_map_group)
+  (#target1: Type0)
+  (#target_size1: target1 -> nat)
+  (#p1: map_group_parser_spec source1 target_size1)
+  (s1: map_group_serializer_spec p1)
+  (#source2: det_map_group)
+  (#target2: Type0)
+  (#target_size2: target2 -> nat)
+  (#p2: map_group_parser_spec source2 target_size2)
+  (s2: map_group_serializer_spec p2 { source1 `map_group3_disjoint` source2 }) // disjointness needed to avoid the CBOR object serialized from one case to be parsed into the other case
+  (target_size: (target1 `either` target2) -> nat {
+    forall x . target_size x == begin match x with
+    | Inl y -> target_size1 y
+    | Inr y -> target_size2 y
+    end
+  })
+: Tot (map_group_serializer_spec (map_group_parser_spec_choice p1 p2 target_size))
+= fun x -> match x with
+  | Inl y -> s1 y
+  | Inr y -> s2 y
+
+let map_group_parser_spec_zero_or_one
+  (#source: det_map_group)
+  (#target: Type)
+  (#target_size: target -> nat)
+  (p: map_group_parser_spec source target_size)
+  (target_size': option target -> nat {
+    forall x . target_size' x == begin match x with
+    | None -> 0
+    | Some x -> target_size x
+    end
+  })
+: Tot (map_group_parser_spec (map_group3_zero_or_one source) target_size')
+= fun x ->
+    if Some? (source x)
+    then Some (p x)
+    else None
+
+let map_group_serializer_spec_zero_or_one
+  (#source: nonempty_map_group) // needed because the empty case must map to None only
+  (#target: Type)
+  (#target_size: target -> nat)
+  (#p: map_group_parser_spec source target_size)
+  (s: map_group_serializer_spec p)
+  (target_size': option target -> nat {
+    forall x . target_size' x == begin match x with
+    | None -> 0
+    | Some x -> target_size x
+    end
+  })
+: Tot (map_group_serializer_spec (map_group_parser_spec_zero_or_one p target_size'))
+= fun x ->
+    match x with
+    | None -> []
+    | Some y -> s y
